Simplify and annotate cache
- Commit to a single protocol, for only the cache. It is unlikely we
  will need too much more than this for the concurrency bit, and it will
  be easiest to do caching, locking and hiding readers together without
  a bunch of interfaces and subprotocols.
- Add ghost update annotations for all the existing functions

src/ConcurrentCache.v
@@ -2,6 +2,7 @@ Require Import CoopConcur.
 Require Import CoopConcurAuto.
 Require Import Protocols.
 Require Import Locking.
+Require Import DiskReaders.
 Require Import Star.
 Import List.ListNotations.
 Import Hlist.HlistNotations.
@@ -10,22 +11,19 @@ Require Import MemCache.
 
 Section ConcurrentCache.
 
-  Variable Sigma:State.
-
-  Definition CacheSigma := defState [Flags; Cache] [Locks addr; Cache; DISK].
-
-  Variable cacheProj : StateProj Sigma CacheSigma.
+  Definition Sigma := defState [Flags; Cache] [Locks addr; Cache; DISK].
 
   (* memory variables *)
-
-  Definition mLocks := ltac:(hget 0 (memVars cacheProj)).
-  Definition mCache := ltac:(hget 1 (memVars cacheProj)).
+  Definition mLocks : var (mem_types Sigma) _ := ltac:(hmember 0 (mem_types Sigma)).
+  Definition mCache : var (mem_types Sigma) _ := ltac:(hmember 1 (mem_types Sigma)).
 
   (* abstraction ("virtual") variables *)
-
-  Definition vLocks := ltac:(hget 0 (abstractionVars cacheProj)).
-  Definition vCache := ltac:(hget 1 (abstractionVars cacheProj)).
-  Definition vDisk := ltac:(hget 2 (abstractionVars cacheProj)).
+  Definition vLocks : var (abstraction_types Sigma) _
+    := ltac:(hmember 0 (abstraction_types Sigma)).
+  Definition vCache : var (abstraction_types Sigma) _
+    := ltac:(hmember 1 (abstraction_types Sigma)).
+  Definition vDisk : var (abstraction_types Sigma) _
+    := ltac:(hmember 2 (abstraction_types Sigma)).
 
   Definition cacheR (tid:TID) : Relation Sigma :=
     fun s s' =>
@@ -48,8 +46,6 @@ Section ConcurrentCache.
       locks_rep (addr_lock (get mLocks m)) (get vLocks s) /\
       cache_rep d (get vCache s) (get vDisk s).
 
-  Variable delta:Protocol Sigma.
-
   Hint Resolve same_domain_refl.
   Hint Resolve lock_protocol_refl.
 
@@ -63,48 +59,53 @@ Section ConcurrentCache.
     admit.
   Admitted.
 
-  Definition CacheProtocol : Protocol Sigma :=
+  Definition delta : Protocol Sigma :=
     defProtocol cacheI cacheR cacheR_trans_closed.
-
-  Hypothesis cacheProtocolDerive : SubProtocol delta CacheProtocol.
-  Hypothesis cacheProtocolRespected : SubProtocolUnder
-                                        (privateVars [( mLocks; mCache )] [( vLocks; vCache )])
-                                        CacheProtocol delta.
 
   Definition cache_maybe_read {T} a rx : prog Sigma T :=
     c <- Get mCache;
       rx (cache_val c a).
 
   Definition cache_write {T} a v rx : prog Sigma T :=
+    tid <- GetTID;
     c <- Get mCache;
       let c' := cache_add c a (Dirty v) in
-      Assgn mCache c';;
-            rx tt.
+      _ <- Assgn mCache c';
+        _ <- var_update vCache
+          (* fix cache *)
+          (fun c => cache_add c a (Dirty v));
+        _ <- var_update vDisk
+          (* update virtual disk *)
+          (fun vd => upd vd a (v, Some tid));
+        rx tt.
 
-  (* TODO: add ghost updates for reader state *)
   Definition AsyncRead {T} a rx : prog Sigma T :=
-    StartRead a;;
-              Yield a;;
-              v <- FinishRead a;
+    tid <- GetTID;
+      _ <- StartRead a;
+      _ <- var_update vDisk
+        (fun vd => add_reader vd a tid);
+      _ <- Yield a;
+      v <- FinishRead a;
+      _ <- var_update vDisk
+        (fun vd => remove_reader vd a);
       rx v.
 
   Definition lock {T} (a: addr) rx : prog Sigma T :=
     tid <- GetTID;
-      wait_for mLocks (is_open #a) a;;
-               l <- Get mLocks;
-      Assgn mLocks (set_locked l #a);;
-            GhostUpdate
-            (fun s =>
-               let l := get vLocks s in
-               let l' := upd_lock l a (Owned tid) in
-               set vLocks l' s);;
-            rx tt.
+      _ <- wait_for mLocks (is_open #a) a;
+      l <- Get mLocks;
+      _ <- Assgn mLocks (set_locked l #a);
+      _ <- var_update vLocks
+        (fun l => upd_lock l a (Owned tid));
+      rx tt.
 
   Definition cache_fill {T} a rx : prog Sigma T :=
     v <- AsyncRead a;
       c <- Get mCache;
       let c' := cache_add c a (Clean v) in
-      Assgn mCache c';;
-            rx tt.
+      _ <- Assgn mCache c';
+        _ <- var_update vCache
+          (fun c => cache_add c a (Clean v));
+        rx tt.
 
 End ConcurrentCache.
